Classes/SoundMonad.v
@@ -1,0 +1,24 @@
+Require Export Base.
+Require Import Classes.Monad.
+Require Import Classes.Functor.
+Require Import Classes.Applicative.
+Require Import Classes.Galois.
+Require Import Instances.Monad.
+Require Import Instances.Preorder.
+Require Import Instances.Galois.
+
+Section monad_sound. 
+  Context (M M' : Type → Type) `{Monad M, Monad M'}.
+  Context {A A' B B' : Type} `{Galois A A', Galois B B'}.
+  Context `{Galois (M A) (M' A'), Galois (M B) (M' B')}.
+  Context `{Galois (M (A → B)) (M' (A' → B'))}.
+
+  Class SoundMonads : Type :=
+  {
+    fmap_sound : gamma (fmap (Functor:=H2)) (fmap);
+    pure_sound : gamma (pure (Applicative:=H3)) (pure);
+    app_sound  : gamma (app (Applicative:=H3)) (app);
+    bind_sound : gamma (bindM (Monad:=H4)) (bindM) ;
+  }.
+End monad_sound.
+Hint Resolve fmap_sound pure_sound app_sound bind_sound : soundness.
